theories/simulations/msim/Tactics.v
@@ -1,32 +1,32 @@
-(* From iris.proofmode Require Import proofmode. *)
-(* Require Import Common. *)
-(* Require Import FSpec ISim WSim. *)
-(* Require Export TacticsCommon ITactics WTactics. *)
+From iris.proofmode Require Import proofmode.
+Require Import Common.
+Require Import FSpec ISim WSim.
+Require Export TacticsCommon ITactics WTactics.
 
-(* Tactic Notation "iwcase" tactic(itac) tactic(wtac) := *)
-(*   match goal with *)
-(*   | [ |- environments.envs_entails _ (isim _ _ _ _ _ _ _ _ _ _ _) ] => itac *)
-(*   | [ |- environments.envs_entails _ (wsim _ _ _ _ _ _ _ _ _ _ _ _ _) ] => wtac *)
-(*   end. *)
+Tactic Notation "iwcase" tactic(itac) tactic(wtac) :=
+  match goal with
+  | [ |- environments.envs_entails _ (isim _ _ _ _ _ _ _ _ _ _ _) ] => itac
+  | [ |- environments.envs_entails _ (wsim _ _ _ _ _ _ _ _ _ _ _ _ _) ] => wtac
+  end.
 
-(* Ltac step_l := iwcase (do 1 istep_l) (do 1 wstep_l). *)
-(* Ltac steps_l := iwcase (do 1 isteps_l) (do 1 wsteps_l). *)
+Ltac step_l := iwcase (do 1 istep_l) (do 1 wstep_l).
+Ltac steps_l := iwcase (do 1 isteps_l) (do 1 wsteps_l).
 
-(* Ltac step_r := iwcase (do 1 istep_r) (do 1 wstep_r). *)
-(* Ltac steps_r := iwcase (do 1 isteps_r) (do 1 wsteps_r). *)
+Ltac step_r := iwcase (do 1 istep_r) (do 1 wstep_r).
+Ltac steps_r := iwcase (do 1 isteps_r) (do 1 wsteps_r).
 
-(* Ltac step := iwcase (do 1 istep) (do 1 wstep). *)
+Ltac step := iwcase (do 1 istep) (do 1 wstep).
 
-(* Tactic Notation "force_l" := iwcase (do 1 iforce_l) (do 1 wforce_l). *)
-(* Tactic Notation "force_l" uconstr(p) := iwcase (do 1 iforce_l p) (do 1 wforce_l p). *)
-(* Ltac forces_l := iwcase (do 1 iforces_l) (do 1 wforces_l). *)
+Tactic Notation "force_l" := iwcase (do 1 iforce_l) (do 1 wforce_l).
+Tactic Notation "force_l" uconstr(p) := iwcase (do 1 iforce_l p) (do 1 wforce_l p).
+Ltac forces_l := iwcase (do 1 iforces_l) (do 1 wforces_l).
 
-(* Tactic Notation "force_r" := iwcase (do 1 iforce_r) (do 1 wforce_r). *)
-(* Tactic Notation "force_r" uconstr(p) := iwcase (do 1 iforce_r p) (do 1 wforce_r p). *)
-(* Ltac forces_r := iwcase (do 1 iforces_r) (do 1 wforces_r). *)
+Tactic Notation "force_r" := iwcase (do 1 iforce_r) (do 1 wforce_r).
+Tactic Notation "force_r" uconstr(p) := iwcase (do 1 iforce_r p) (do 1 wforce_r p).
+Ltac forces_r := iwcase (do 1 iforces_r) (do 1 wforces_r).
 
-(* Ltac inline_l := iwcase (do 1 iinline_l) (do 1 winline_l). *)
-(* Ltac inline_r := iwcase (do 1 iinline_r) (do 1 winline_r). *)
+Ltac inline_l := iwcase (do 1 iinline_l) (do 1 winline_l).
+Ltac inline_r := iwcase (do 1 iinline_r) (do 1 winline_r).
 
 (* Ltac call hyps := iwcase (do 1 icall hyps) (do 1 wcall hyps). *)
 
